theories/stdpp_img.v
@@ -1,8 +1,7 @@
 (** This is a concept missing from stdpp, an image/codomain set for maps
     Hopefully it will get merged into stdpp and we can remove this from here.
     https://gitlab.mpi-sws.org/iris/stdpp/-/merge_requests/444 *)
-From Coq Require Import ssreflect.
-From stdpp Require Import countable gmap list.
+From stdpp Require Import fin_maps.
 
 (** The function [img m] should yield the image/codomain of [m]. That is a finite
 set of type [D] that contains the values that appear in [m].
@@ -14,35 +13,39 @@ Global Instance: Params (@img) 3 := {}.
 Global Arguments img : clear implicits.
 Global Arguments img {_ _ _} !_ / : simpl nomatch, assert.
 
+Global Instance fin_map_img K A M D
+  `{FinMapToList K A M, Singleton A D, Empty D, Union D}
+  : Img M D := map_to_set (λ _ a, a).
 
-Class FinMapImg K A M D
-  `{Img (M A) D, FMap M,
-    ∀ A, Lookup K A (M A), ∀ A, Empty (M A), ∀ A, PartialAlter K A (M A),
-    OMap M, Merge M, ∀ A, FinMapToList K A (M A), EqDecision K,
-    ElemOf A D, Empty D, Singleton A D,
-    Union D, Intersection D, Difference D} := {
-  finmap_img_map :> FinMap K M;
-  finmap_img_set :> Set_ A D;
-  elem_of_img (m:M A) (v:A) : v ∈ img m <-> ∃ (k:K), m !! k = Some v
-}.
 
-Section fin_map_img.
-  Context `{FinMapImg K A M D}.
-  Implicit Types (m:M A) (k:K) (v:A).
-  Infix "≡" := (@equiv D _) (at level 70).
+(** ** The [img] (image/codomain) operation *)
+Section image.
+  Context `{FinMap K M, FinSet A D}.
+  Implicit Types (m : M A) (k : K) (v : A).
 
-  Lemma elem_of_img_2 m k v: m !! k = Some v -> v ∈ img m.
+  (* avoid writing ≡@{D} everywhere... *)
+  Notation img := (@img (M A) D _).
+
+  Lemma elem_of_img m v : v ∈ img m ↔ ∃ (k : K), m !! k = Some v.
+  Proof.
+    unfold img, fin_map_img. rewrite elem_of_map_to_set. split.
+    - intros (k & v' & mk_v' & v'_v). exists k. rewrite v'_v in mk_v'. exact mk_v'.
+    - intros [k mk_v]. exists k. exists v. split; [exact mk_v|reflexivity].
+  Qed.
+
+  Lemma elem_of_img_2 m k v : m !! k = Some v → v ∈ img m.
   Proof. intros Hmkv. rewrite elem_of_img. exists k. exact Hmkv. Qed.
 
-  Lemma not_elem_of_img m v: v ∉ img m <-> ∀ k, m !! k ≠ Some v.
-  Proof. rewrite elem_of_img. split.
-    intros Hm k Hk. contradiction (Hm (ex_intro _ k Hk)).
-    intros Hm [k Hk]. contradiction (Hm k Hk).
+  Lemma not_elem_of_img m v : v ∉ img m ↔ ∀ k, m !! k ≠ Some v.
+  Proof.
+    rewrite elem_of_img. split.
+    - intros Hm k Hk. contradiction (Hm (ex_intro _ k Hk)).
+    - intros Hm [k Hk]. contradiction (Hm k Hk).
   Qed.
-  Lemma not_elem_of_img_1 m v k: v ∉ img m -> m !! k ≠ Some v.
+  Lemma not_elem_of_img_1 m v k : v ∉ img m → m !! k ≠ Some v.
   Proof. intros Hm. apply not_elem_of_img. exact Hm. Qed.
 
-  Lemma subseteq_img (m1 m2:M A): m1 ⊆ m2 -> img m1 ⊆ img m2.
+  Lemma subseteq_img m1 m2 : m1 ⊆ m2 → img m1 ⊆ img m2.
   Proof.
     intros Hm v Hv. rewrite elem_of_img.
     apply elem_of_img in Hv as [k Hv]. exists k.
@@ -50,256 +53,258 @@ Section fin_map_img.
     apply (Hm k v Hv).
   Qed.
 
-  Lemma img_filter (P : K * A → Prop) `{!∀ x, Decision (P x)} m (X:D):
+  Lemma img_filter (P : K * A → Prop) `{!∀ x, Decision (P x)} m (X : D) :
     (∀ v, v ∈ X ↔ ∃ k, m !! k = Some v ∧ P (k, v)) →
     img (filter P m) ≡ X.
   Proof.
-    intros HX i. rewrite elem_of_img HX.
+    intros HX i. rewrite elem_of_img, HX.
     unfold is_Some. by setoid_rewrite map_filter_lookup_Some.
   Qed.
-  Lemma img_filter_subseteq (P : K * A → Prop) `{!∀ x, Decision (P x)} m:
+  Lemma img_filter_subseteq (P : K * A → Prop) `{!∀ x, Decision (P x)} m :
     img (filter P m) ⊆ img m.
   Proof. apply subseteq_img, map_filter_subseteq. Qed.
 
-  Lemma img_empty: img (∅ : M A) ≡ ∅.
+  Lemma img_empty : img ∅ ≡ ∅.
   Proof.
     rewrite set_equiv. intros x. split; intros Hempty.
-    apply elem_of_img in Hempty. destruct Hempty as [k Hk].
-    rewrite lookup_empty in Hk. discriminate.
-    rewrite elem_of_empty in Hempty. contradiction Hempty.
+    - apply elem_of_img in Hempty. destruct Hempty as [k Hk].
+      rewrite lookup_empty in Hk. discriminate.
+    - rewrite elem_of_empty in Hempty. contradiction Hempty.
   Qed.
-  Lemma img_empty_iff m: img m ≡ ∅ ↔ m = ∅.
+  Lemma img_empty_iff m : img m ≡ ∅ ↔ m = ∅.
   Proof.
     split; [|intros ->; by rewrite img_empty].
     intros E. apply map_empty. intros i.
-    destruct (m!!i) eqn:Hm. apply elem_of_img_2 in Hm. set_solver.
-    reflexivity.
+    destruct (m!!i) eqn:Hm.
+    - apply elem_of_img_2 in Hm. set_solver.
+    - reflexivity.
   Qed.
-  Lemma img_empty_inv m: img m ≡ ∅ → m = ∅.
+  Lemma img_empty_inv m : img m ≡ ∅ → m = ∅.
   Proof. apply img_empty_iff. Qed.
 
-  Lemma img_insert k v m: img (<[k:=v]> m) ⊆ {[ v ]} ∪ img m.
+  Lemma img_insert k v m : img (<[k:=v]> m) ⊆ {[ v ]} ∪ img m.
   Proof.
     intros w Hw. apply elem_of_img in Hw as [k' Hw].
     apply lookup_insert_Some in Hw as [[Hkk' Hvw] | [Hkk' Hmk']].
-    apply elem_of_union_l, elem_of_singleton. symmetry. apply Hvw.
-    apply elem_of_union_r, elem_of_img. exists k'. apply Hmk'.
+    - apply elem_of_union_l, elem_of_singleton. symmetry. apply Hvw.
+    - apply elem_of_union_r, elem_of_img. exists k'. apply Hmk'.
   Qed.
-  Lemma elem_of_img_insert k v m: v ∈ img (<[k:=v]> m).
+  Lemma elem_of_img_insert k v m : v ∈ img (<[k:=v]> m).
   Proof. apply elem_of_img. exists k. apply lookup_insert. Qed.
-  Lemma elem_of_img_insert_ne k v w m: v ≠ w -> w ∈ img(<[k:=v]> m) -> w ∈ img m.
-  Proof. rewrite !elem_of_img. intros Hv [k' Hk].
-    destruct (decide (k=k')) as [Heq|Heq]. rewrite Heq lookup_insert in Hk.
-    apply Some_inj in Hk. contradiction (Hv Hk).
-    rewrite lookup_insert_ne in Hk. exact Heq. exists k'. exact Hk.
-  Qed.
-  Lemma img_insert_notin k v m: m!!k = None -> img (<[k:=v]> m) ≡ {[ v ]} ∪ img m.
+  Lemma elem_of_img_insert_ne k v w m : v ≠ w → w ∈ img(<[k:=v]> m) → w ∈ img m.
   Proof.
-    intros Hm w. rewrite elem_of_union !elem_of_img elem_of_singleton.
+    rewrite !elem_of_img. intros Hv [k' Hk].
+    destruct (decide (k=k')) as [Heq|Heq].
+    - rewrite Heq, lookup_insert in Hk.
+      apply Some_inj in Hk. contradiction (Hv Hk).
+    - rewrite (lookup_insert_ne _ _ _ _ Heq) in Hk. exists k'. exact Hk.
+  Qed.
+  Lemma img_insert_notin k v m : m!!k = None → img (<[k:=v]> m) ≡ {[ v ]} ∪ img m.
+  Proof.
+    intros Hm w. rewrite elem_of_union, !elem_of_img, elem_of_singleton.
     setoid_rewrite lookup_insert_Some.
     split.
-    intros [k' [[Hk Hv] | [Hk Hv]]]. left. done. right. exists k'. done.
-    intros [Hv | [k' Hv]]. exists k. left. done. exists k'. right.
-    destruct (decide (k=k')) as [Hk|Hk]. simplify_eq. done.
+    - intros [k' [[Hk Hv] | [Hk Hv]]]; [ (left; done) | right]. exists k'. done.
+    - intros [Hv | [k' Hv]]; [ (exists k; left; done) | (exists k'; right) ].
+      destruct (decide (k=k')) as [Hk|Hk]; [ simplify_eq | done ].
   Qed.
 
-  Lemma img_singleton k v : img ({[ k := v ]} : M A) ≡ {[ v ]}.
+  Lemma img_singleton k v : img {[ k := v ]} ≡ {[ v ]}.
   Proof.
     rewrite set_equiv. intros x.
     rewrite elem_of_img. rewrite elem_of_singleton.
     setoid_rewrite lookup_singleton_Some. set_solver.
   Qed.
 
-  Lemma elem_of_img_union m1 m2 v:
-    v ∈ img (m1 ∪ m2) ->
-    v ∈ img m1 \/ v ∈ img m2.
+  Lemma elem_of_img_union m1 m2 v :
+    v ∈ img (m1 ∪ m2) →
+    v ∈ img m1 ∨ v ∈ img m2.
   Proof.
     intros Hv12.
     (* destruct (elem_of_img (m1 ∪ m2) v) as . *)
     rewrite (elem_of_img (m1 ∪ m2) v) in Hv12.
     destruct Hv12 as [k Hv12].
     destruct (lookup_union_Some_raw m1 m2 k v) as [Hspec _].
-    destruct (Hspec Hv12) as [Hm | [_ Hm]].
-    left. 2: right.
-    all: rewrite elem_of_img; exists k; exact Hm.
+    destruct (Hspec Hv12) as [Hm | [_ Hm]];
+    [ left | right ]; rewrite elem_of_img; exists k; exact Hm.
   Qed.
-  Lemma img_union_subseteq m1 m2: img (m1 ∪ m2) ⊆ img m1 ∪ img m2.
+  Lemma elem_of_img_union_l m1 m2 v :
+    v ∈ img m1 → v ∈ img (m1 ∪ m2).
+  Proof.
+    intros Hv. rewrite elem_of_img. apply elem_of_img in Hv as [k Hv].
+    exists k. by apply lookup_union_Some_l.
+  Qed.
+  Lemma elem_of_img_union_r m1 m2 v :
+    m1 ##ₘ m2 → v ∈ img m2 → v ∈ img (m1 ∪ m2).
+  Proof.
+    intros Hdisj Hv. rewrite elem_of_img. apply elem_of_img in Hv as [k Hv].
+    exists k. by apply lookup_union_Some_r.
+  Qed.
+  Lemma elem_of_img_union_disjoint m1 m2 v :
+    m1 ##ₘ m2 → v ∈ img (m1 ∪ m2) ↔ v ∈ img m1 \/ v ∈ img m2.
+  Proof.
+    intros Hdisj. split.
+    - apply elem_of_img_union.
+    - intros [Hv | Hv].
+      + by apply elem_of_img_union_l.
+      + by apply elem_of_img_union_r.
+  Qed.
+
+  Lemma img_union_subseteq m1 m2 : img (m1 ∪ m2) ⊆ img m1 ∪ img m2.
   Proof. intros v Hv. apply elem_of_union, elem_of_img_union. exact Hv. Qed.
-  Lemma img_union_subseteq_l m1 m2: img m1 ⊆ img (m1 ∪ m2).
+  Lemma img_union_subseteq_l m1 m2 : img m1 ⊆ img (m1 ∪ m2).
+  Proof. intros v Hv. by apply elem_of_img_union_l. Qed.
+  Lemma img_union_subseteq_r m1 m2 : m1 ##ₘ m2 → img m2 ⊆ img (m1 ∪ m2).
+  Proof. intros Hdisj v Hv. by apply elem_of_img_union_r. Qed.
+  Lemma img_union_disjoint m1 m2 : m1 ##ₘ m2 → img (m1 ∪ m2) ≡ img m1 ∪ img m2.
   Proof.
-    intros v Hv. apply elem_of_img in Hv as [k Hv].
-    rewrite elem_of_img.
-    exists k. apply lookup_union_Some_l. apply Hv.
+    intros Hdisj. apply set_equiv. intros v.
+    rewrite elem_of_union. by apply elem_of_img_union_disjoint.
   Qed.
 
-  Lemma img_fmap `{Img (M B) D2, ElemOf B D2, Empty D2, Singleton B D2, Union D2, Intersection D2, Difference D2, !FinMapImg K B M D2}
-        `{Elements A D, EqDecision A, !FinSet A D} (f: A -> B) m:
-    img (f <$> m) ≡@{D2} set_map f (img m).
+  Lemma img_finite m : set_finite (img m).
   Proof.
-    apply set_equiv. intros v. rewrite elem_of_img elem_of_map.
-    split. intros [k Hk]. rewrite lookup_fmap in Hk.
-    destruct (m!!k) as [a|] eqn:Hm. exists a. split. apply Some_inj in Hk. done.
-    apply elem_of_img_2 in Hm. done. discriminate.
-    intros [a [Ha Hm]]. apply elem_of_img in Hm as [k Hk]. exists k.
-    rewrite lookup_fmap Hk Ha. reflexivity.
-  Qed.
-
-  Lemma img_kmap `{Img (M2 A) D, FinMap K2 M2, !FinMapImg K2 A M2 D}
-        (f: K -> K2) `{!Inj (=) (=) f} m:
-    img (kmap (M2:=M2) f m) ≡ img m.
-  Proof.
-    apply set_equiv. intros v.
-    split; intros Hv; rewrite elem_of_img; apply elem_of_img in Hv as [k Hv].
-    apply lookup_kmap_Some in Hv as [k' [Hk' Hv]]. exists k'. done. done.
-    exists (f k). rewrite lookup_kmap. done.
-  Qed.
-
-  Lemma img_finite m: set_finite (img m).
-  Proof.
-    induction m using map_ind.
+    induction m as [|x i m Hm IHm] using map_ind .
     - rewrite img_empty. apply empty_finite.
-    - apply (set_finite_subseteq _ _ (img_insert i x m)).
-      apply union_finite. apply singleton_finite. apply IHm.
+    - apply (set_finite_subseteq _ _ (img_insert x i m)).
+      apply union_finite; [ apply singleton_finite | apply IHm ].
   Qed.
 
-  Lemma img_list_to_map l:
-    (∀ k v v', (k,v) ∈ l -> (k,v') ∈ l -> v = v') ->
-    img (list_to_map l : M A) ≡ list_to_set l.*2.
+  Lemma img_list_to_map l :
+    (∀ k v v', (k,v) ∈ l → (k,v') ∈ l → v = v') →
+    img (list_to_map l) ≡ list_to_set l.*2.
   Proof.
-    induction l as [|?? IH].
+    induction l as [|a l IH].
     - by rewrite img_empty.
     - intros Hl. destruct a as [k v]. simpl.
-      assert (IH': img (list_to_map l: M A) ≡ list_to_set l.*2).
+      assert (IH' : img (list_to_map l) ≡ list_to_set l.*2).
       { apply IH. intros k' v' v'' Hv' Hv''. apply (Hl k' v' v''); apply elem_of_list_further; assumption. }
-      rewrite -IH'.
+      rewrite <- IH'.
       destruct ((list_to_map l : M A)!!k) as [w|] eqn:Hw.
-      assert (Hvw: v = w). apply (Hl k). apply elem_of_list_here.
-      apply elem_of_list_further. apply elem_of_list_to_map_2. exact Hw.
-      rewrite -Hvw in Hw.
-      apply set_equiv. intros x. split.
-      intros Hx. apply img_insert in Hx. done.
-      intros Hx. apply elem_of_union in Hx as [Hv | Hx].
-      apply elem_of_singleton in Hv. rewrite Hv. apply elem_of_img_insert.
-      apply elem_of_img in Hx as [k' Hx].
-      destruct (decide (k=k')). simplify_eq. apply elem_of_img_insert.
-      apply elem_of_img. exists k'. rewrite lookup_insert_ne; assumption.
-      rewrite img_insert_notin. exact Hw. reflexivity.
+      + assert (Hvw : v = w).
+        { apply (Hl k); [ apply elem_of_list_here | apply elem_of_list_further ].
+          apply elem_of_list_to_map_2. exact Hw. }
+        rewrite <- Hvw in Hw. apply set_equiv. intros x. split.
+        * intros Hx. apply img_insert in Hx. done.
+        * intros Hx. apply elem_of_union in Hx as [Hv | Hx].
+          -- apply elem_of_singleton in Hv. rewrite Hv. apply elem_of_img_insert.
+          -- apply elem_of_img in Hx as [k' Hx].
+             destruct (decide (k=k'));  [(simplify_eq; apply elem_of_img_insert)|].
+              apply elem_of_img. exists k'. rewrite lookup_insert_ne; assumption.
+      + rewrite img_insert_notin; [reflexivity | exact Hw].
   Qed.
 
   (** Alternative definition of [img] in terms of [map_to_list]. *)
-  Lemma img_alt m: img m ≡ list_to_set (map_to_list m).*2.
+  Lemma img_alt m : img m ≡ list_to_set (map_to_list m).*2.
   Proof.
     rewrite <-(list_to_map_to_list m) at 1.
-    rewrite img_list_to_map.
+    rewrite img_list_to_map; [reflexivity|].
     intros k v v' Hv Hv'. rewrite !elem_of_map_to_list in Hv, Hv'.
     rewrite Hv in Hv'. apply Some_inj. exact Hv'.
-    done.
   Qed.
 
-  Lemma img_singleton_inv m v:
-    img m ≡ {[ v ]} -> ∀ k, m !! k = None \/ m !! k = Some v.
+  Lemma img_singleton_inv m v :
+    img m ≡ {[ v ]} → ∀ k, m !! k = None ∨ m !! k = Some v.
   Proof.
     intros Hm k. destruct (m!!k) eqn:Hmk.
-    right. apply elem_of_img_2 in Hmk. rewrite Hm elem_of_singleton in Hmk.
-    rewrite Hmk. reflexivity.
-    left. reflexivity.
+    - right. apply elem_of_img_2 in Hmk. rewrite Hm, elem_of_singleton in Hmk.
+      rewrite Hmk. reflexivity.
+    - left. reflexivity.
   Qed.
 
-  Lemma img_union_inv `{!RelDecision (∈@{D})} X Y m:
-    X ## Y ->
-    img m ≡ X ∪ Y ->
-    ∃ m1 m2, m = m1 ∪ m2 /\ m1 ##ₘ m2 /\ img m1 ≡ X /\ img m2 ≡ Y.
+  Lemma img_union_inv `{!RelDecision (∈@{D})} X Y m :
+    X ## Y →
+    img m ≡ X ∪ Y →
+    ∃ m1 m2, m = m1 ∪ m2 ∧ m1 ##ₘ m2 ∧ img m1 ≡ X ∧ img m2 ≡ Y.
   Proof.
     intros Hsep Himg.
     exists (filter (λ '(_,x), x ∈ X) m), (filter (λ '(_,x), x ∉ X) m).
-    assert (Hdisj: filter (λ '(_, x), x ∈ X) m ##ₘ filter (λ '(_, x), x ∉ X) m).
+    assert (Hdisj : filter (λ '(_, x), x ∈ X) m ##ₘ filter (λ '(_, x), x ∉ X) m).
     { apply map_disjoint_filter_complement. }
     split_and!.
     - symmetry. apply map_filter_union_complement.
     - apply Hdisj.
     - apply img_filter; intros v; split; [|naive_solver].
-      intros Hv. apply (union_subseteq_l X Y) in Hv as Hv'. rewrite -Himg elem_of_img in Hv'.
+      intros Hv. apply (union_subseteq_l X Y) in Hv as Hv'. rewrite <-Himg, elem_of_img in Hv'.
       destruct Hv' as [k Hk]. exists k. done.
     - apply img_filter; intros v; split.
       + intros Hv.
-        apply (union_subseteq_r X Y) in Hv as Hv'. rewrite -Himg elem_of_img in Hv'.
-        destruct Hv' as [k Hk]. exists k. split. done.
-        destruct (decide (v ∈ X)) as [Hx|Hx]. contradiction (Hsep v Hx Hv). done.
+        apply (union_subseteq_r X Y) in Hv as Hv'. rewrite <-Himg, elem_of_img in Hv'.
+        destruct Hv' as [k Hk]. exists k. split; [done|].
+        destruct (decide (v ∈ X)) as [Hx|Hx]; [contradiction (Hsep v Hx Hv)| done].
       + intros (k&Hk&Hv). apply elem_of_img_2 in Hk. set_solver.
   Qed.
 
   Section Leibniz.
     Context `{!LeibnizEquiv D}.
 
-    Lemma img_empty_L: img (@empty (M A) _) = ∅.
+    Lemma img_empty_L : img ∅ = ∅.
     Proof. unfold_leibniz. exact img_empty. Qed.
 
-    Lemma img_empty_iff_L m: img m = ∅ ↔ m = ∅.
+    Lemma img_empty_iff_L m : img m = ∅ ↔ m = ∅.
     Proof. unfold_leibniz. apply img_empty_iff. Qed.
-    Lemma img_empty_inv_L m: img m = ∅ → m = ∅.
+    Lemma img_empty_inv_L m : img m = ∅ → m = ∅.
     Proof. apply img_empty_iff_L. Qed.
 
-    Lemma img_singleton_L k v: img ({[ k := v ]} : M A) = {[ v ]}.
+    Lemma img_singleton_L k v : img {[ k := v ]} = {[ v ]}.
     Proof. unfold_leibniz. apply img_singleton. Qed.
 
-    Lemma img_insert_notin_L k v m: m!!k=None -> img (<[k:=v]> m) = {[ v ]} ∪ img m.
+    Lemma img_insert_notin_L k v m : m!!k=None → img (<[k:=v]> m) = {[ v ]} ∪ img m.
     Proof. unfold_leibniz. apply img_insert_notin. Qed.
 
-    Lemma img_fmap_L `{Img (M B) D2, ElemOf B D2, Empty D2, Singleton B D2, Union D2, Intersection D2, Difference D2, !FinMapImg K B M D2}
-          `{Elements A D, EqDecision A, !FinSet A D, !LeibnizEquiv D2} (f: A -> B) m:
-      img (f <$> m) = set_map f (img m).
-    Proof. unfold_leibniz. apply img_fmap. Qed.
+    Lemma img_union_disjoint_L m1 m2 : m1 ##ₘ m2 → img (m1 ∪ m2) = img m1 ∪ img m2.
+    Proof. unfold_leibniz. apply img_union_disjoint. Qed.
 
-    Lemma img_kmap_L `{Img (M2 A) D, FinMap K2 M2, !FinMapImg K2 A M2 D}
-          (f: K -> K2) `{!Inj (=) (=) f} m:
-      img (kmap (M2:=M2) f m) = img m.
-    Proof. unfold_leibniz. apply img_kmap. done. Qed.
-
-    Lemma img_list_to_map_L l:
-      (∀ k v v', (k,v) ∈ l -> (k,v') ∈ l -> v = v') ->
-      img (list_to_map l : M A) = list_to_set l.*2.
+    Lemma img_list_to_map_L l :
+      (∀ k v v', (k,v) ∈ l → (k,v') ∈ l → v = v') →
+      img (list_to_map l) = list_to_set l.*2.
     Proof. unfold_leibniz. apply img_list_to_map. Qed.
 
-    Lemma img_alt_L m: img m = list_to_set (map_to_list m).*2.
+    Lemma img_alt_L m : img m = list_to_set (map_to_list m).*2.
     Proof. unfold_leibniz. apply img_alt. Qed.
 
-    Lemma img_singleton_inv_L m v:
-      img m = {[ v ]} -> ∀ k, m !! k = None \/ m !! k = Some v.
+    Lemma img_singleton_inv_L m v :
+      img m = {[ v ]} → ∀ k, m !! k = None ∨ m !! k = Some v.
     Proof. unfold_leibniz. apply img_singleton_inv. Qed.
 
-    Lemma img_union_inv_L `{!RelDecision (∈@{D})} X Y m:
-      X ## Y ->
-      img m = X ∪ Y ->
-      ∃ m1 m2, m = m1 ∪ m2 /\ m1 ##ₘ m2 /\ img m1 = X /\ img m2 = Y.
+    Lemma img_union_inv_L `{!RelDecision (∈@{D})} X Y m :
+      X ## Y →
+      img m = X ∪ Y →
+      ∃ m1 m2, m = m1 ∪ m2 ∧ m1 ##ₘ m2 ∧ img m1 = X ∧ img m2 = Y.
     Proof. unfold_leibniz. apply img_union_inv. Qed.
   End Leibniz.
 
   (** * Set solver instances *)
   Global Instance set_unfold_img_empty i : SetUnfoldElemOf i (img (∅:M A)) False.
-  Proof. constructor. by rewrite img_empty elem_of_empty. Qed.
-End fin_map_img.
+  Proof. constructor. by rewrite img_empty, elem_of_empty. Qed.
+End image.
 
-Global Instance fin_map_img K A M D
-  `{FinMapToList K A M, Singleton A D, Empty D, Union D}
-: Img M D := map_to_set (fun _ a => a).
-Global Instance gmap_img K A
-  `{EqDecision K, Countable K, EqDecision A, Countable A}
-: Img (gmap K A) (gset A) := fin_map_img K A (gmap K A) (gset A).
-
-Global Instance fin_map_img_spec K A M D
-  `{HFinMap:FinMap K M} `{HFinSet:FinSet A D} : FinMapImg K A M D.
+Lemma img_fmap `{FinMap K M, FinSet A D, FinSet B D2} (f : A → B) (m : M A) :
+  img (f <$> m) ≡@{D2} set_map (C:=D) f (img m).
 Proof.
-  split.
-  exact HFinMap.
-  apply fin_set_set.
-  unfold img, fin_map_img.
-  intros m v.
-  rewrite elem_of_map_to_set.
-  split.
-  intros [k [v' [mk_v' v'_v]]]. exists k. rewrite v'_v in mk_v'. exact mk_v'.
-  intros [k mk_v]. exists k. exists v. split. exact mk_v. reflexivity.
+  apply set_equiv. intros v. rewrite elem_of_img, elem_of_map. split.
+  - intros [k Hk]. rewrite lookup_fmap in Hk.
+    destruct (m!!k) as [a|] eqn:Hm; [|discriminate].
+    exists a. split.
+    + apply Some_inj in Hk. done.
+    + apply (elem_of_img_2 (D:=D)) in Hm. done.
+  - intros [a [Ha Hm]]. apply elem_of_img in Hm as [k Hk].
+    exists k. rewrite lookup_fmap, Hk, Ha. reflexivity.
 Qed.
+Lemma img_fmap_L `{FinMap K M, FinSet A D, FinSet B D2, !LeibnizEquiv D2} (f : A → B) (m : M A) :
+  img (f <$> m) = set_map (C:=D) (D:=D2) f (img m).
+Proof. unfold_leibniz. apply img_fmap. Qed.
 
-Global Instance gmap_imp_spec K A
- `{EqDecision K, Countable K, EqDecision A, Countable A}
-: FinMapImg K A (gmap K) (gset A) := fin_map_img_spec K A (gmap K) (gset A).
+Lemma img_kmap `{FinMap K M, FinMap K2 M2, FinSet A D}
+      (f : K → K2) `{!Inj (=) (=) f} m :
+  img (kmap (M2:=M2) f m) ≡@{D} img m.
+Proof.
+  apply set_equiv. intros v.
+  split; intros Hv; rewrite elem_of_img; apply elem_of_img in Hv as [k Hv].
+  - apply lookup_kmap_Some in Hv as [k' [Hk' Hv]]; [exists k'|]; done.
+  - exists (f k). rewrite lookup_kmap; done.
+Qed.
+Lemma img_kmap_L `{FinMap K M, FinMap K2 M2, FinSet A D, !LeibnizEquiv D}
+  (f : K → K2) `{!Inj (=) (=) f} m :
+  img (kmap (M2:=M2) f m) = (img m : D).
+Proof. unfold_leibniz. apply img_kmap. done. Qed.
